reorganizing

proofs/x86-64/avx2/ml_dsa_65/encoding/gamma1.ec
@@ -1,85 +1,18 @@
 require import AllCore List IntDiv RealExp.
 
 from Jasmin require import JModel_x86.
-require import Bindings JWordList.
+require import Bindings.
 
 from JazzEC require import Ml_dsa_65_avx2.
-from JazzEC require import Array16 Array256 Array640 WArray1024 WArray16.
-from Spec require import GFq Rq Serialization Conversion.
-import BitEncoding.
-import BitChunking.
+from JazzEC require import Array256 Array640.
+from Spec require import GFq Rq Serialization Conversion Parameters MLDSA_W32_Rep.
+import BitEncoding BitChunking.
 
 import CDR Round Zq.
 
-type wpoly = W32.t Array256.t.
-
-op liftu_wpoly (pw : wpoly) : poly =
-  map (fun w => incoeff (W32.to_uint w)) pw.
-
-op lifts_wpoly (pw : wpoly) : poly =
-  map (fun w => incoeff (W32.to_sint w)) pw.
-
-op unlift_poly (p : poly) : wpoly = map (fun c => W32.of_int (asint c)) p.
-
-op poly_urng(b : int, p : poly) = all (fun i => 0 <= asint i < b) p.
-op poly_srng(bl bh : int, p : poly) = all (fun i => -bl <= as_sint i <= bh) p.
-
-op wpoly_urng(b : int, pw : wpoly) = all (fun i => 0 <= W32.to_uint i < b) pw.
-op wpoly_srng(bl bh : int, pw : wpoly) = all (fun i => -bl <= W32.to_sint i <= bh) pw.
-
-(* natural spec and precondition *)
-op gamma1 : int = 524288. (* 2**19 *) 
-
-(* Circuit spec and precondition *)
-
-op pre_gamma1_encode_polynomial(c : W32.t) = 
-    (W32_sub (W32.zero) (W32.of_int (524287))) \sle c /\ c \sle W32.of_int gamma1. 
-
-op gamma1_encode_polynomial_lane(c : W32.t) : W20.t = 
-    truncateu_32_20 (W32_sub (W32.of_int gamma1) c).
-
-import Parameters.
-
+require import ArrayExtra JWord_extra (* w2bitsE as int2bs *) EclibExtra (* size_flatten' *) JWordList (* nth_chunk *).
  
-(* Move to array theory *)
-lemma all_tolist ['a] (p : 'a -> bool) (a : 'a Array256.t) :
-  (Array256.all p a) <=> (List.all p (to_list a)) by 
-  rewrite /all !allP /to_list /mkseq /=;split => H x Hx; 
-   [have /# := mapP ("_.[_]" a) (iota_ 0 n) x | smt(mapP)].
-   
-lemma all_imply ['a] (p q : 'a -> bool) (s : 'a Array256.t) :
-  (forall x, p x => q x) => all p s => all q s
-  by rewrite /all !allP /to_list /mkseq /= => H x Hx;smt(mapP).
-
-lemma array256_mapE ['a 'b] (f : 'a -> 'b) (a : 'a Array256.t) :
-  Array256.to_list (Array256.map f a) = List.map f (Array256.to_list a).
-  rewrite /all /to_list /mkseq /= -{1}map_comp /(\o) /=.
-  apply (eq_from_nth witness);1: by rewrite !size_map.
-  move => i;rewrite !size_map size_iota /max /= => ib.
-  rewrite !(nth_map witness) /=;1,2:smt(size_map size_iota).
-  by rewrite /map initiE /=;1:by rewrite nth_iota /#.
-qed.
-  
-lemma array256_map_comp ['a 'b 'c] (f : 'a -> 'b) (g : 'b -> 'c) (a : 'a Array256.t) :
-  Array256.map g ((Array256.map f a)) = Array256.map (fun x => g (f x)) a
-  by rewrite /map tP => i ib;smt(Array256.initiE).
-
-lemma array256_allP ['a] (p : 'a -> bool) (a : 'a Array256.t) :
-  Array256.all p a <=> (forall x, x \in Array256.to_list a => p x).
-proof. by rewrite all_tolist allP. qed.
-(* *)
-
-(* move to list theory *)
-lemma in_map_id ['a] (f : 'a -> 'a) (s : 'a list) :
-  (forall x, x \in s => f x = x) => map f s = s.
-proof. by move=> id_f; rewrite -{2}[s]map_id &(eq_in_map). qed.
-
-lemma in_map_cancel ['a 'b] (f : 'a -> 'b) (g : 'b -> 'a) (s : 'a list) :
-  (forall x, x \in s => g (f x) = x) => map g (map f s) = s.
-proof. by move=> can_fg; rewrite -map_comp in_map_id. qed.
-
-(* *)
-
+(* Words of weird size should be cloned and bound here. *)
 lemma truncateu_32_20E (w : W32.t) : truncateu_32_20 w = W20.bits2w (take 20 (W32.w2bits w)).
 proof.
 rewrite /truncateu_32_20 W20.of_intE W32.to_uintE BS2Int.bs2int_mod //;congr.
@@ -87,26 +20,36 @@ have {1}-> : gamma1_bits = size (take gamma1_bits (w2bits w)) by rewrite size_ta
 by rewrite BS2Int.bs2intK.
 qed.
 
-lemma w2bitsE (w : W32.t) : w2bits w = BS2Int.int2bs 32 (W32.to_uint w).
-proof. rewrite to_uintE;smt(W32.size_w2bits BS2Int.bs2intK). qed.
+op sigextu_20_32(a : W20.t) : W32.t = W32.of_int (to_sint a).
+bind op [W20.t & W32.t] sigextu_20_32 "sextend".
+realize bvsextendP.
+move => bv;rewrite  /sigextu_20_32 /to_sint /smod /= !of_uintK /=.
+case (524288 <= to_uint bv); 2: smt(W20.to_uint_cmp).
+have ? : 2^20 = 1048576 by auto => />.
+move =>?;rewrite -{2}(oppzK (to_uint bv - 1048576)) modNz /=; smt(W20.to_uint_cmp). 
+qed.
+realize le_size by done.
 
-lemma map_W8_w2bits_cancel (s : bool list list) :
-     (forall bs, bs \in s => size bs = 8)
-  => map W8.w2bits (map W8.bits2w s) = s.
-proof.
-by move=> h; rewrite in_map_cancel // => bs /h; apply: W8.bits2wK.
+lemma to_sint_uint_rng_pos_20(xx : W20.t) :
+    0 <= to_sint xx  <=> 0 <= to_uint xx < 524288.
+ have /= Hxx := W20.to_uint_cmp xx. 
+ rewrite /to_sint /smod /= /#.
 qed.
 
-abbrev a256_w20_tobits (a : W20.t Array256.t) : bool list =
-  flatten (List.map (W20.w2bits) (Array256.to_list a)).
+lemma to_sint_uint_rng_neg_20(xx : W20.t) :
+    to_sint xx < 0  <=> 524288 <= to_uint xx <1048576.
+ have /= Hxx := W20.to_uint_cmp xx. 
+ rewrite /to_sint /smod /= /#.
+qed.
 
-abbrev l640_w8_ofbits (a : bool list) : W8.t list =
-  List.map W8.bits2w (chunk 8 a).
+(* Circuit spec *)
 
-abbrev a640_w8_ofbits (a : bool list) : W8.t Array640.t =
-  Array640.of_list witness (l640_w8_ofbits a).
-
+op gamma1 : int = 524288. (* 2**19 *) 
 lemma ilog_gamma1 : ilog 2 (gamma1 - 1 + gamma1) = 19 by rewrite /gamma1 /=.
+
+op gamma1_encode_polynomial_lane(c : W32.t) : W20.t = 
+    truncateu_32_20 (W32_sub (W32.of_int gamma1) c).
+
  
 lemma BitPack_liftE (p : wpoly) :
   wpoly_srng (gamma1 - 1) gamma1 p =>
@@ -115,7 +58,7 @@ lemma BitPack_liftE (p : wpoly) :
              init_array640_w8 (fun i => W8.init (fun j => mapped.[(i*8+j) %/ 20].[(i*8+j) %% 20]))).
 proof.
 move=> h @/BitPack; (pose l := ilog 2 _) => /=.
-have ? := ilog_gamma1.
+have Hlog := ilog_gamma1.
 have ? : size
   (flatten (map (fun (x : W32.t) => IntegerToBits (Top.gamma1 - as_sint (incoeff (to_sint x))) (l + 1)) (to_list p))) = 256*20.
 +  rewrite  (size_flatten_ctt (l+1)).
@@ -140,10 +83,9 @@ move: h => @/wpoly_srng /array256_allP /(_ v _) //= /=.
 + rewrite /to_list /mkseq mapP; exists ((i * 8 + j) %/ gamma1_bits); smt(mem_iota).
 move => h. 
 rewrite incoeffK_sint_small 1:/# /W32_sub truncateu_32_20E get_bits2w 1:/#.
-rewrite nth_take 1,2:/#. 
-rewrite /IntegerToBits w2bitsE.
+rewrite nth_take 1,2:/# w2bitsE. 
 have  -> := BS2Int.int2bs_cat 20 32 (to_uint (W32.of_int Top.gamma1 - v)) _;1:smt().
-rewrite nth_cat ifT;1: by rewrite BS2Int.size_int2bs /#.
+rewrite /IntegerToBits nth_cat ifT;1: by rewrite BS2Int.size_int2bs /#.
 congr;2:smt().
 congr;1:smt(). 
 have := (W32.of_uintK (Top.gamma1 - to_sint v)).
@@ -153,9 +95,8 @@ rewrite W32.of_intN;congr.
 rewrite /to_sint /smod /=.
 case (2147483648 <= to_uint v) => ?;last by smt(W32.to_uintK pow2_32).
 move : h; rewrite /to_sint /smod ifT //= => ?.
-by smt(@W32 pow2_32).  
+congr;rewrite to_uint_eq of_uintK /=;smt(W32.to_uint_cmp pow2_32). 
 qed.
-
 
 lemma gamma1_encode_polynomial _a :
    hoare [ M.gamma1____encode_polynomial :
@@ -193,20 +134,8 @@ conseq (:  _ ==>
 
 qed.
 
-op pre_gamma1_decode_to_polynomial(c : W20.t) = true.
-
 op gamma1_decode_to_polynomial_lane(c : W20.t) : W32.t = 
     (W32_sub (W32.of_int gamma1) (zeroextu_20_32 c)).
-
-
-abbrev l640_w8_tobits (a : W8.t Array640.t) : bool list  =
-  flatten (List.map W8.w2bits (to_list a)).
-
-abbrev l256_w20_ofbits (a : bool list) :  W20.t list   =
-  List.map W20.bits2w (chunk 20 a).
-
-abbrev a256_w20_ofbits (a : bool list) :  W20.t Array256.t   =
-  Array256.of_list witness (l256_w20_ofbits a).
 
 
 lemma BitUnack_liftE (bytes : W8.t Array640.t) :
@@ -231,7 +160,7 @@ rewrite (nth_map []) /=.
   rewrite (EclibExtra.size_flatten' 8);1: by smt(mapP W8.size_w2bits).
   by rewrite size_map size_to_list /= /#.
 congr; rewrite  /gamma1_decode_to_polynomial_lane /W32_sub.
-rewrite ilog_gamma1 /= /zeroextu_20_32. print nth_chunk.
+rewrite ilog_gamma1 /= /zeroextu_20_32. 
 rewrite nth_chunk // 1:/#.
 + rewrite /BytesToBits. 
   rewrite (EclibExtra.size_flatten' 8);1: by smt(mapP W8.size_w2bits).
@@ -263,6 +192,7 @@ rewrite (nth_flatten false 8).
 rewrite (nth_map witness) /=; 1: by rewrite size_to_list /#.
 by rewrite initiE 1:/# /=.
 qed.
+
 
 lemma gamma1_decode_to_polynomial _a :
    hoare [ M.gamma1____decode_to_polynomial :
@@ -307,29 +237,12 @@ qed.
 
 import VecMat PolyLVec.
 
-type wpolylvec = wpoly LArray.t. 
-
-op liftu_wpolylvec(wv : wpolylvec) : polylvec =
-  map liftu_wpoly wv.
-
-op lifts_wpolylvec (wv : wpolylvec) : polylvec =
-  map lifts_wpoly wv.
-
-op unlift_polylvec (v : polylvec) : wpolylvec = map unlift_poly v.
-
-op polylvec_urng(p : polylvec, b : int) = all (poly_urng b) p.
-op polylvec_srng(p : polylvec, bl bh : int) = all (poly_srng bl bh) p.
-
-op wpolylvec_urng(pw : wpolylvec, b : int) = all (wpoly_urng b) pw.
-op wpolylvec_srng(pw : wpolylvec, bl bh : int) = all (wpoly_srng bl bh) pw.
-
 require import Array1280 Array3200.
 
 op  input_unflatten(a : 'a Array3200.t) =
      LArray.init (fun i => Array640.of_list witness (sub a (640*i) 640)).
 op  output_unflatten(a : 'a Array1280.t) =
      LArray.init (fun i => Array256.of_list witness (sub a (256*i) 256)).
-        
 
 lemma gamma1_decode _a :
     lvec = 5 =>
